chore: remove `Mutable` and fix `UnionFind` API (#97)
Remove `Mutable`, as we could not find a design that supports `UnionFind` over polymorphic index types without running into the [polymorphic references](https://counterexamples.org/polymorphic-references.html) problem.

AlgorithmTest/UnionFind.lean
@@ -2,28 +2,101 @@ import Algorithm.Data.UnionFind
 
 abbrev UF := UnionFind (Fin 10) (Vector (Fin 10) 10) (Vector Nat 10)
 
-/--
-info: 1
-2
--/
-#guard_msgs in #eval show IO Unit from do
-  let mut uf : UF := default
-  IO.println (uf.find 1)
-  uf := uf.union 1 2
-  uf := uf.union 3 4
-  uf := uf.union 2 4
-  IO.println ((Quot.unquot (Mutable.get uf)).val.parent[(1 : Fin 10)])
+abbrev UFImpl := UnionFindImpl.UnionFindWF (Fin 10) (Vector (Fin 10) 10) (Vector Nat 10)
+
+def initialUF : UFImpl := ⟨default, UnionFindImpl.UnionFind.default_wf⟩
 
 /--
 info: 1
 4
 4
+4
+1
 -/
 #guard_msgs in #eval show IO Unit from do
-  let mut uf : UF := default
-  IO.println (uf.find 1)
+  let initial : UF := default
+  IO.println (initial.find 1).fst
+  let uf := ((initial.union 1 2).union 3 4).union 2 4
+  let result := uf.find 1
+  IO.println result.fst
+  IO.println (result.snd.find 1).fst
+  IO.println (result.snd.size result.fst (uf.find_isRoot 1))
+  IO.println (initial.find 1).fst
+
+-- The result/state convention can be used directly with `modifyGet`.
+def findInState (i : Fin 10) : StateM UF (Fin 10) :=
+  modifyGet (fun uf ↦ uf.find i)
+
+example (uf : UF) (i : Fin 10) : (findInState i).run uf = uf.find i := rfl
+
+example (x : UFImpl) (i : Fin 10) :
+    (⟦(x.find i).snd⟧ : UF) = ⟦x⟧ :=
+  Quotient.sound (x.find_snd_root i)
+
+-- Inspect representatives in this runtime test to check that compression is retained.
+/--
+info: 2
+4
+4
+2
+-/
+#guard_msgs in #eval show IO Unit from do
+  let initial : UF := default
+  let uf := ((initial.union 1 2).union 3 4).union 2 4
+  IO.println ((Quot.unquot uf).val.parent[(1 : Fin 10)])
+  let (r, compressed) := uf.find 1
+  IO.println r
+  IO.println ((Quot.unquot compressed).val.parent[(1 : Fin 10)])
+  IO.println ((Quot.unquot uf).val.parent[(1 : Fin 10)])
+
+/--
+info: 1
+2
+-/
+#guard_msgs in #eval show IO Unit from do
+  let mut uf := initialUF
+  IO.println (uf.find 1).fst
   uf := uf.union 1 2
   uf := uf.union 3 4
   uf := uf.union 2 4
-  IO.println (uf.find 1)
-  IO.println ((Quot.unquot (Mutable.get uf)).val.parent[(1 : Fin 10)])
+  IO.println (uf.val.parent[(1 : Fin 10)])
+
+/--
+info: 1
+4
+4
+2
+4
+1
+-/
+#guard_msgs in #eval show IO Unit from do
+  let mut uf := initialUF
+  IO.println (uf.find 1).fst
+  uf := uf.union 1 2
+  uf := uf.union 3 4
+  uf := uf.union 2 4
+  let (r, compressed) := uf.find 1
+  IO.println r
+  IO.println (compressed.val.parent[(1 : Fin 10)])
+  -- Path compression affects only the returned forest.
+  IO.println (uf.val.parent[(1 : Fin 10)])
+  IO.println (compressed.size (compressed.root 1) (.root _ _))
+  -- Unions also preserve the original forest.
+  IO.println (initialUF.find 1).fst
+
+-- Merging already connected nodes must retain compression from both searches.
+/--
+info: 8
+8
+2
+6
+8
+-/
+#guard_msgs in #eval show IO Unit from do
+  let uf := ((((((initialUF.union 1 2).union 3 4).union 2 4).union 5 6).union 7 8).union 6 8).union 4 8
+  let compressed := uf.union 1 5
+  IO.println (compressed.val.parent[(1 : Fin 10)])
+  IO.println (compressed.val.parent[(5 : Fin 10)])
+  IO.println (uf.val.parent[(1 : Fin 10)])
+  IO.println (uf.val.parent[(5 : Fin 10)])
+  IO.println (compressed.size (compressed.root 1) (.root _ _))
