Algorithm.lean
@@ -18,7 +18,6 @@ import Algorithm.Data.Graph.AdjList
 import Algorithm.Data.Graph.IsDFSForest
 import Algorithm.Data.HashMap
 import Algorithm.Data.HashSet
-import Algorithm.Data.MutableQuotient
 import Algorithm.Data.PairingHeap
 import Algorithm.Data.UnionFind
 import Algorithm.Graph.DFS
